LTS_v2

reg2nfa.thy
@@ -35,7 +35,7 @@ primrec len_reg :: "'v regexp \<Rightarrow> nat" where
 primrec trans2LTS :: "'v regexp \<Rightarrow> 'v set \<Rightarrow> (('v regexp \<times> 'v set \<times> 'v regexp) set * ('v regexp * 'v regexp) set)" where 
     "trans2LTS (LChr v) alp_set= ({(LChr v,{v},\<epsilon>)},{})"|
     "trans2LTS (ESet) alp_set= ({(ESet,{},\<epsilon>)},{})"|
-    "trans2LTS (\<epsilon>) alp_set = ({(\<epsilon>,{},\<epsilon>)},{})"|
+    "trans2LTS (\<epsilon>) alp_set = ({},{(\<epsilon>,\<epsilon>)})"|
     "trans2LTS (Dot) alp_set = ({(Dot ,alp_set, \<epsilon>)},{})"|
     "trans2LTS (Concat r1 r2) alp_set =(renameDelta1 (fst (trans2LTS r1 alp_set)) (ConcatRegexp r2) \<union> (fst (trans2LTS r2 alp_set)),
                                         (renameDelta2 (snd (trans2LTS r1 alp_set)) (ConcatRegexp r2) \<union> {(Concat \<epsilon> r2, r2)}  \<union> snd (trans2LTS r2 alp_set)))"|
@@ -73,6 +73,18 @@ section "function correctness of transition from regexp expression to  nondeterm
 lemma [simp]:"0 < len_reg r" 
   by (induct r) auto
  
+lemma [simp]:"(\<epsilon>, q'') \<in> snd (trans2LTS r v) \<Longrightarrow> q'' = \<epsilon>"
+  apply (induct r) apply auto
+  done
+
+lemma "(Ques r, p) \<in> (snd (trans2LTS r v)) \<Longrightarrow> False"
+  apply(induct r)
+  apply auto
+
+lemma [simp]:"(\<epsilon>, \<sigma>, q'') \<in> fst (trans2LTS r v) \<Longrightarrow> False"
+  apply(induct r)
+  apply auto
+  done
 
 lemma "(q, q') = trans2LTS r1 v \<Longrightarrow> \<forall>(a,b) \<in> q'. len_reg a < len_reg (Alter r1 r2)"
   apply(induction r1 arbitrary:r2)
@@ -87,65 +99,6 @@ lemma "(q, q') = trans2LTS r1 v \<Longrightarrow> \<forall>(a,b) \<in> q'. len_r
   subgoal for r2 by auto
   done
 
-lemma "LTS_is_reachable (fst (trans2LTS r1 v), insert (Alter r1 r2, r1) (snd (trans2LTS r1 v))) (Alter r1 r2) x ε \<Longrightarrow> 
-       LTS_is_reachable (fst (trans2LTS r1 v),insert (Alter r1 r2, r1) (snd (trans2LTS r1 v))) r1 x ε"
-  proof (induction rule: LTS_is_reachable.cases)
-    case (LTS_Empty lts q)
-    then show ?case apply auto done
-  next
-    case (LTS_Step1 q q'' lts l q')
-    then show ?case apply auto 
-    proof -
-      assume 1:"x = l"
-      assume 2:"lts = (fst (trans2LTS r1 v), insert (Alter r1 r2, r1) (snd (trans2LTS r1 v)))"
-      assume 3:"q = Alter r1 r2"
-      assume 4:"q' = ε"
-      assume 5:"LTS_is_reachable (fst (trans2LTS r1 v), insert (Alter r1 r2, r1) (snd (trans2LTS r1 v))) q'' l ε"
-      assume 6:"(Alter r1 r2, q'') ∈ snd (trans2LTS r1 v)"
-      show "LTS_is_reachable (fst (trans2LTS r1 v), insert (Alter r1 r2, r1) (snd (trans2LTS r1 v))) r1 l ε " proof -
-        have 7:"(Alter r1 r2, q'') ∈ snd (trans2LTS r1 v) \<Longrightarrow> False" 
-          apply(induction r1) 
-          subgoal by auto
-          subgoal for x by auto
-          subgoal for r11 r12 apply auto sorry
-          subgoal for r11 r12 apply auto sorry
-          subgoal by auto
-          subgoal for r1 by auto
-          subgoal for r1 by auto
-          subgoal for r1 apply auto sorry
-          subgoal by auto done
-      then have 8:"False"  using "6" by blast
-      thus ?thesis  by blast
-    qed
-  qed
-  next
-    case (LTS_Step2 a q lts w q')
-    then show ?case apply auto  subgoal for q''  σ proof - 
-    assume a1:"x = a # w"
-    assume a2:"lts = (fst (trans2LTS r1 v), insert (Alter r1 r2, r1) (snd (trans2LTS r1 v)))"
-    assume a3:"q = Alter r1 r2"
-    assume a4:"q' = ε"
-    assume a5:"a ∈ σ"
-    assume a6:"(Alter r1 r2, σ, q'') ∈ fst (trans2LTS r1 v)"
-    assume a7:"LTS_is_reachable (fst (trans2LTS r1 v), insert (Alter r1 r2, r1) (snd (trans2LTS r1 v))) q'' w ε" 
-    show "∃q'' σ. a ∈ σ ∧ (r1, σ, q'') ∈ fst (trans2LTS r1 v) ∧ LTS_is_reachable (fst (trans2LTS r1 v), insert (Alter r1 r2, r1) (snd (trans2LTS r1 v))) q'' w ε" 
-    proof -
-      have c1:"(Alter r1 r2, σ, q'') ∈ fst (trans2LTS r1 v) \<Longrightarrow> False" 
-        apply(induction r1)
-        subgoal by auto
-        subgoal for x by auto
-        subgoal for r11 r12 apply auto sorry
-        subgoal for r11 r12 apply auto sorry
-        subgoal by auto 
-        subgoal for r1 by auto
-        subgoal for r1 by auto
-        subgoal for r1 apply auto sorry
-        subgoal by auto done
-      then show ?thesis using a6 by blast
-      qed
-    qed
-    done
-qed
 
 theorem uniqueInitalState:"\<I> (reg2nfa r v) = {r}"
   apply (induct r)
@@ -173,10 +126,14 @@ next
       apply auto
       subgoal for w
       proof -
-        assume a1:" LTS_is_reachable ({(LChr x, {x}, \<epsilon>)}, {}) \<epsilon> w \<epsilon>"
-        from a1 have "w = []" 
-          by(rule LTS_is_reachable.cases)auto
-        then show "w=[]" .
+        assume a1:"LTS_is_reachable {(LChr x, {x}, \<epsilon>)} {} (LChr x) (x # w) \<epsilon>"
+        from a1 show "w = []" 
+          apply(rule LTS_is_reachable.cases) apply auto
+        proof -
+          assume "LTS_is_reachable {(LChr x, {x}, \<epsilon>)} {} \<epsilon> w \<epsilon>"
+          from this show "w = []"
+            by (rule LTS_is_reachable.cases) auto
+        qed
       qed 
       done
     next
@@ -190,7 +147,7 @@ next
       apply auto
       subgoal for a w
       proof -
-        assume a1:"LTS_is_reachable ({(Dot, v, \<epsilon>)}, {}) \<epsilon> w \<epsilon>"
+        assume a1:"LTS_is_reachable {(Dot, v, \<epsilon>)} {} \<epsilon> w \<epsilon>"
         from a1 have "w=[]"       
           by (rule LTS_is_reachable.cases) auto
         then show "w=[]" .
@@ -203,7 +160,7 @@ next
     apply (unfold \<L>_def  NFA_accept_def)
     apply auto
     subgoal for x
-    by(rule LTS_is_reachable.cases) auto
+      by (rule LTS_is_reachable.cases) auto
   done
 next
   case (Alter r1 r2)
@@ -212,73 +169,66 @@ next
     apply auto
     subgoal for x
     proof -
-      assume a1:"sem_reg r1 v = {w. LTS_is_reachable (trans2LTS r1 v) r1 w \<epsilon>}"
-      assume a2:"sem_reg r2 v = {w. LTS_is_reachable (trans2LTS r2 v) r2 w \<epsilon>}"
-      assume a3:"LTS_is_reachable (trans2LTS r1 v) r1 x \<epsilon>"
-      then show "LTS_is_reachable (fst (trans2LTS r1 v) \<union> fst (trans2LTS r2 v), insert (Alter r1 r2, r1) (insert (Alter r1 r2, r2) (snd (trans2LTS r1 v) \<union> snd (trans2LTS r2 v)))) (Alter r1 r2) x \<epsilon>"
+      assume a1:"sem_reg r1 v = {w. LTS_is_reachable (fst (trans2LTS r1 v)) (snd (trans2LTS r1 v)) r1 w \<epsilon>}"
+      assume a2:"sem_reg r2 v = {w. LTS_is_reachable (fst (trans2LTS r2 v)) (snd (trans2LTS r2 v)) r2 w \<epsilon>}"
+      assume a3:"LTS_is_reachable (fst (trans2LTS r1 v)) (snd (trans2LTS r1 v)) r1 x \<epsilon>"
+      then show "LTS_is_reachable (fst (trans2LTS r1 v) \<union> fst (trans2LTS r2 v)) (insert (Alter r1 r2, r1) (insert (Alter r1 r2, r2) (snd (trans2LTS r1 v) \<union> snd (trans2LTS r2 v)))) (Alter r1 r2) x \<epsilon>"
      proof -
-        have c1:"LTS_is_reachable (fst (trans2LTS r1 v) \<union> fst (trans2LTS r2 v), insert (Alter r1 r2, r1) (insert (Alter r1 r2, r2) (snd (trans2LTS r1 v) \<union> snd (trans2LTS r2 v)))) (Alter r1 r2) [] r1" 
-          by (metis LTS_Empty LTS_Step1 insertI1 snd_conv)
-        from a3 have c2:"LTS_is_reachable (fst (trans2LTS r1 v) \<union> fst (trans2LTS r2 v), insert (Alter r1 r2, r1) (insert (Alter r1 r2, r2) (snd (trans2LTS r1 v) \<union> snd (trans2LTS r2 v)))) r1 x \<epsilon>"
+        have c1:"LTS_is_reachable (fst (trans2LTS r1 v) \<union> fst (trans2LTS r2 v)) (insert (Alter r1 r2, r1) (insert (Alter r1 r2, r2) (snd (trans2LTS r1 v) \<union> snd (trans2LTS r2 v)))) (Alter r1 r2) [] r1" 
+          by (metis LTS_Empty LTS_Step1 insertI1)
+        from a3 have c2:"LTS_is_reachable (fst (trans2LTS r1 v) \<union> fst (trans2LTS r2 v)) (insert (Alter r1 r2, r1) (insert (Alter r1 r2, r2) (snd (trans2LTS r1 v) \<union> snd (trans2LTS r2 v)))) r1 x \<epsilon>"
           by (metis Un_insert_right subLTSlemma)
-        from c1 c2 have "LTS_is_reachable (fst (trans2LTS r1 v) \<union> fst (trans2LTS r2 v), insert (Alter r1 r2, r1) (insert (Alter r1 r2, r2) (snd (trans2LTS r1 v) \<union> snd (trans2LTS r2 v)))) (Alter r1 r2) x \<epsilon>"
-          by (metis LTS_Step1 insertI1 snd_eqD)
+        from c1 c2 have "LTS_is_reachable (fst (trans2LTS r1 v) \<union> fst (trans2LTS r2 v)) (insert (Alter r1 r2, r1) (insert (Alter r1 r2, r2) (snd (trans2LTS r1 v) \<union> snd (trans2LTS r2 v)))) (Alter r1 r2) x \<epsilon>"
+          by (metis LTS_Step1 insertI1)
         then show ?thesis by auto
       qed
     qed
      subgoal for x
       proof -
-      assume a1:"sem_reg r1 v = {w. LTS_is_reachable (trans2LTS r1 v) r1 w \<epsilon>} "
-      assume a2:"sem_reg r2 v = {w. LTS_is_reachable (trans2LTS r2 v) r2 w \<epsilon>}"
-      assume a3:"LTS_is_reachable (trans2LTS r2 v) r2 x \<epsilon>"
-      then show "LTS_is_reachable (fst (trans2LTS r1 v) \<union> fst (trans2LTS r2 v), insert (Alter r1 r2, r1) (insert (Alter r1 r2, r2) (snd (trans2LTS r1 v) \<union> snd (trans2LTS r2 v)))) (Alter r1 r2) x \<epsilon>"
+      assume a1:"sem_reg r1 v = {w. LTS_is_reachable (fst (trans2LTS r1 v)) (snd (trans2LTS r1 v)) r1 w \<epsilon>}"
+      assume a2:"sem_reg r2 v = {w. LTS_is_reachable (fst (trans2LTS r2 v)) (snd (trans2LTS r2 v)) r2 w \<epsilon>}"
+      assume a3:"LTS_is_reachable (fst (trans2LTS r2 v)) (snd (trans2LTS r2 v)) r2 x \<epsilon>"
+      then show "LTS_is_reachable (fst (trans2LTS r1 v) \<union> fst (trans2LTS r2 v)) (insert (Alter r1 r2, r1) (insert (Alter r1 r2, r2) (snd (trans2LTS r1 v) \<union> snd (trans2LTS r2 v)))) (Alter r1 r2) x \<epsilon>"
       proof -
-        have c1:"LTS_is_reachable (fst (trans2LTS r1 v) \<union> fst (trans2LTS r2 v), insert (Alter r1 r2, r1) (insert (Alter r1 r2, r2) (snd (trans2LTS r1 v) \<union> snd (trans2LTS r2 v)))) (Alter r1 r2) [] r2" 
-          by (metis LTS_Empty LTS_Step1 insertI1 insertI2 snd_eqD)
-        have c2:"LTS_is_reachable (fst (trans2LTS r1 v) \<union> fst (trans2LTS r2 v), insert (Alter r1 r2, r1) (insert (Alter r1 r2, r2) (snd (trans2LTS r1 v) \<union> snd (trans2LTS r2 v)))) r2 x \<epsilon>"
-          using a3 
-          by (smt (z3) Un_commute Un_insert_right subLTSlemma)
-        have "LTS_is_reachable (fst (trans2LTS r1 v) \<union> fst (trans2LTS r2 v), insert (Alter r1 r2, r1) (insert (Alter r1 r2, r2) (snd (trans2LTS r1 v) \<union> snd (trans2LTS r2 v)))) (Alter r1 r2) x \<epsilon>"
-          using c1 c2 
-          by (metis LTS_Step1 insertI1 insertI2 snd_eqD)
+        have c1:"LTS_is_reachable (fst (trans2LTS r1 v) \<union> fst (trans2LTS r2 v)) (insert (Alter r1 r2, r1) (insert (Alter r1 r2, r2) (snd (trans2LTS r1 v) \<union> snd (trans2LTS r2 v))))  (Alter r1 r2) [] r2" 
+          by (metis LTS_Empty LTS_Step1 insertI1 insertI2)
+        have c2:"LTS_is_reachable (fst (trans2LTS r1 v) \<union> fst (trans2LTS r2 v)) (insert (Alter r1 r2, r1) (insert (Alter r1 r2, r2) (snd (trans2LTS r1 v) \<union> snd (trans2LTS r2 v))))  r2 x \<epsilon>"
+          using a3 by (smt (z3) Un_commute Un_insert_right subLTSlemma)
+        have "LTS_is_reachable (fst (trans2LTS r1 v) \<union> fst (trans2LTS r2 v)) (insert (Alter r1 r2, r1) (insert (Alter r1 r2, r2) (snd (trans2LTS r1 v) \<union> snd (trans2LTS r2 v))))  (Alter r1 r2) x \<epsilon>"
+          using c1 c2 by (metis LTS_Step1 insertI1 insertI2)
         then show ?thesis by auto
        qed
      qed
      subgoal for x
      proof -
-       assume a1:"sem_reg r1 v = {w. LTS_is_reachable (trans2LTS r1 v) r1 w ε}"
-       assume a2:"sem_reg r2 v = {w. LTS_is_reachable (trans2LTS r2 v) r2 w ε}"
-       assume a3:"LTS_is_reachable (fst (trans2LTS r1 v) ∪ fst (trans2LTS r2 v), insert (Alter r1 r2, r1) (insert (Alter r1 r2, r2) (snd (trans2LTS r1 v) ∪ snd (trans2LTS r2 v)))) (Alter r1 r2) x ε"
-       assume a4:"¬ LTS_is_reachable (trans2LTS r2 v) r2 x ε" 
-       let ?trans = "(fst (trans2LTS r1 v) ∪ fst (trans2LTS r2 v), insert (Alter r1 r2, r1) (insert (Alter r1 r2, r2) (snd (trans2LTS r1 v) ∪ snd (trans2LTS r2 v))))"
-       from a3 have c1:"LTS_is_reachable ?trans (Alter r1 r2) [] r1"
-         by (metis LTS_Empty LTS_Step1 insertI1 snd_eqD)
-       from a3 have c2:"LTS_is_reachable ?trans (Alter r1 r2) [] r2"
-         by (metis LTS_Empty LTS_Step1 UnI2 insertI1 insert_def snd_eqD)
-       from a3 c1 c2 have c1:"LTS_is_reachable ?trans r1 x \<epsilon> \<or> LTS_is_reachable ?trans r2 x \<epsilon>"
+       assume a1:"sem_reg r1 v = {w. LTS_is_reachable (fst (trans2LTS r1 v)) (snd (trans2LTS r1 v)) r1 w \<epsilon>}"
+       assume a2:"sem_reg r2 v = {w. LTS_is_reachable (fst (trans2LTS r2 v)) (snd (trans2LTS r2 v)) r2 w \<epsilon>}"
+       assume a3:"LTS_is_reachable (fst (trans2LTS r1 v) \<union> fst (trans2LTS r2 v)) (insert (Alter r1 r2, r1) (insert (Alter r1 r2, r2) (snd (trans2LTS r1 v) \<union> snd (trans2LTS r2 v)))) (Alter r1 r2) x \<epsilon>"
+       assume a4:" \<not> LTS_is_reachable (fst (trans2LTS r2 v)) (snd (trans2LTS r2 v)) r2 x \<epsilon>" 
+       let ?trans1 = "(fst (trans2LTS r1 v) \<union> fst (trans2LTS r2 v))"
+       let ?trans2 = "(insert (Alter r1 r2, r1) (insert (Alter r1 r2, r2) (snd (trans2LTS r1 v) \<union> snd (trans2LTS r2 v))))"
+       from a3 have c1:"LTS_is_reachable ?trans1 ?trans2 (Alter r1 r2) [] r1"
+         by (metis LTS_Empty LTS_Step1 insertI1)
+       from a3 have c2:"LTS_is_reachable ?trans1 ?trans2 (Alter r1 r2) [] r2"
+         by (metis LTS_Empty LTS_Step1 UnI2 insertI1 insert_def)
+       from a3 c1 c2 have c1:"LTS_is_reachable ?trans1 ?trans2 r1 x \<epsilon> \<or> LTS_is_reachable ?trans1 ?trans2 r2 x \<epsilon>"
          apply auto
          proof (induction rule: LTS_is_reachable.cases)
-           case (LTS_Empty lts q)
-           then show ?case apply simp done 
+           case (LTS_Empty \<Delta> \<Delta>' q)
+           then show ?case sorry
          next
-           case (LTS_Step1 q q'' lts l q')
-           then show ?case apply auto sorry 
+           case (LTS_Step1 q q'' \<Delta>' \<Delta> l q')
+           then show ?case sorry
          next
-           case (LTS_Step2 a q lts w q')
-           then show ?case apply simp sorry
+           case (LTS_Step2 a q \<Delta> \<Delta>' w q')
+           then show ?case sorry
          qed
-         have c2:"LTS_is_reachable ?trans r1 x \<epsilon> \<Longrightarrow> LTS_is_reachable (trans2LTS r1 v) r1 x ε"
-           apply(rule LTS_is_reachable.cases)
-           apply simp
-           subgoal for lts q by auto
-           subgoal for q q'' lts l q' apply auto sorry
-           subgoal for a q lts w q' apply auto sorry
-           done
-         have c3:"¬ LTS_is_reachable (trans2LTS r2 v) r2 x ε \<Longrightarrow> ¬ LTS_is_reachable ?trans r2 x \<epsilon>"
+         
+         have c2:"LTS_is_reachable ?trans1 ?trans2 r1 x \<epsilon> \<Longrightarrow> LTS_is_reachable (fst (trans2LTS r1 v)) (snd (trans2LTS r1 v)) r1 x \<epsilon>"
            sorry
-           
-           
-       show "LTS_is_reachable (trans2LTS r1 v) r1 x ε"
+         have c3:"\<not> LTS_is_reachable (fst (trans2LTS r2 v)) (snd (trans2LTS r2 v)) r2 x \<epsilon> \<Longrightarrow> \<not> LTS_is_reachable ?trans1 ?trans2 r2 x \<epsilon>"
+           apply auto sorry
+       show " LTS_is_reachable (fst (trans2LTS r1 v)) (snd (trans2LTS r1 v)) r1 x \<epsilon> "
          using c1 c2 c3 a4 by auto
      qed
    done
@@ -289,77 +239,49 @@ next
     apply auto
     subgoal for q p
     proof -
-    assume a1:"sem_reg r1 v = {w. LTS_is_reachable (trans2LTS r1 v) r1 w \<epsilon>}"
-    assume a2:"sem_reg r2 v = {w. LTS_is_reachable (trans2LTS r2 v) r2 w \<epsilon>}"
-    assume a3:"LTS_is_reachable (trans2LTS r1 v) r1 q \<epsilon>"
-    assume a4:"LTS_is_reachable (trans2LTS r2 v) r2 p \<epsilon>"
-    show "LTS_is_reachable
-     ({(Concat q r2, va, Concat q' r2) |q va q'. (q, va, q') ∈ fst (trans2LTS r1 v)} ∪ fst (trans2LTS r2 v),
-      insert (Concat ε r2, r2) ({(Concat q r2, Concat q' r2) |q q'. (q, q') ∈ snd (trans2LTS r1 v)} ∪ snd (trans2LTS r2 v)))
-     (Concat r1 r2) (q @ p) ε"
+    assume a1:"sem_reg r1 v = {w. LTS_is_reachable (fst (trans2LTS r1 v)) (snd (trans2LTS r1 v)) r1 w \<epsilon>}"
+    assume a2:"sem_reg r2 v = {w. LTS_is_reachable (fst (trans2LTS r2 v)) (snd (trans2LTS r2 v)) r2 w \<epsilon>}"
+    assume a3:"LTS_is_reachable (fst (trans2LTS r1 v)) (snd (trans2LTS r1 v)) r1 q \<epsilon>"
+    assume a4:"LTS_is_reachable (fst (trans2LTS r2 v)) (snd (trans2LTS r2 v)) r2 p \<epsilon>"
+    show "LTS_is_reachable ({(Concat q r2, va, Concat q' r2) |q va q'. (q, va, q') \<in> fst (trans2LTS r1 v)} \<union> fst (trans2LTS r2 v))
+     (insert (Concat \<epsilon> r2, r2) ({(Concat q r2, Concat q' r2) |q q'. (q, q') \<in> snd (trans2LTS r1 v)} \<union> snd (trans2LTS r2 v))) (Concat r1 r2) (q @ p) \<epsilon>"
     proof-
-      have c1:"LTS_is_reachable
-     ({(Concat q r2, va, Concat q' r2) |q va q'. (q, va, q') \<in> fst (trans2LTS r1 v)},({(Concat q r2, Concat q' r2) |q q'. (q, q') \<in> snd (trans2LTS r1 v)})) (Concat r1 r2) q (Concat \<epsilon> r2)"
+      have c1:"LTS_is_reachable ({(Concat q r2, va, Concat q' r2) |q va q'. (q, va, q') \<in> fst (trans2LTS r1 v)})
+     (insert (Concat \<epsilon> r2, r2) ({(Concat q r2, Concat q' r2) |q q'. (q, q') \<in> snd (trans2LTS r1 v)})) (Concat r1 r2) q (Concat \<epsilon> r2)"
         using a3   
         apply (induction rule: LTS_is_reachable.induct)  
-        apply auto
-        apply (metis (mono_tags, lifting) CollectI LTS_Step1 snd_conv)
+          apply auto
+        apply (metis (mono_tags, lifting) LTS_Step1 insertI2 mem_Collect_eq)
         by blast
-      then have c2:"LTS_is_reachable
-     ({(Concat q r2, va, Concat q' r2) |q va q'. (q, va, q') \<in> fst (trans2LTS r1 v)},
-      insert (Concat ε r2, r2) ({(Concat q r2, Concat q' r2) |q q'. (q, q') ∈ snd (trans2LTS r1 v)} ∪ snd (trans2LTS r2 v)))
-             (Concat r1 r2) q (Concat \<epsilon> r2)"
-        apply (induction rule: LTS_is_reachable.cases)
-          subgoal for lts qa
-            by auto
-          subgoal for qa lts l q'
-            apply auto
-            by (smt (z3) Un_commute c1 fst_conv insert_def snd_conv subLTSlemma sup_idem)
-          subgoal for a qa lts w q'
-            apply auto 
-            by (smt (z3) Un_commute Un_insert_left fst_conv snd_conv subLTSlemma sup_idem)
-        done
-      then have c3:"LTS_is_reachable
-           ({(Concat q r2, va, Concat q' r2) |q va q'. (q, va, q') \<in> fst (trans2LTS r1 v)} \<union> fst (trans2LTS r2 v),
-            insert (Concat ε r2, r2) ({(Concat q r2, Concat q' r2) |q q'. (q, q') ∈ snd (trans2LTS r1 v)} ∪ snd (trans2LTS r2 v)))
-            (Concat r1 r2) q (Concat \<epsilon> r2)"
-        by (metis (no_types, lifting) Un_insert_right c1 fst_eqD snd_conv subLTSlemma)
-        have c4:"LTS_is_reachable
-           ({(Concat q r2, va, Concat q' r2) |q va q'. (q, va, q') \<in> fst (trans2LTS r1 v)} \<union> fst (trans2LTS r2 v),
-            insert (Concat ε r2, r2) ({(Concat q r2, Concat q' r2) |q q'. (q, q') ∈ snd (trans2LTS r1 v)} ∪ snd (trans2LTS r2 v)))
-          (Concat \<epsilon> r2) [] r2"
-        by (smt (z3) LTS_Empty LTS_Step1 insertI1 insert_commute snd_conv)
-        have c5:"LTS_is_reachable
-           ({(Concat q r2, va, Concat q' r2) |q va q'. (q, va, q') \<in> fst (trans2LTS r1 v)} \<union> fst (trans2LTS r2 v),
-            insert (Concat ε r2, r2) ({(Concat q r2, Concat q' r2) |q q'. (q, q') ∈ snd (trans2LTS r1 v)} ∪ snd (trans2LTS r2 v)))
-         r2 p \<epsilon>"
-        using a4 
-        by (smt (z3) insert_def subLTSlemma sup.commute sup_left_commute)
-      have "LTS_is_reachable
-           ({(Concat q r2, va, Concat q' r2) |q va q'. (q, va, q') \<in> fst (trans2LTS r1 v)} \<union> fst (trans2LTS r2 v),
-            insert (Concat ε r2, r2) ({(Concat q r2, Concat q' r2) |q q'. (q, q') ∈ snd (trans2LTS r1 v)} ∪ snd (trans2LTS r2 v)))
-           (Concat r1 r2) (q @ p) \<epsilon>" using c3 c4 c5 
-        by (smt (z3) append.right_neutral joinLTSlemma)
+      then have c2:"LTS_is_reachable ({(Concat q r2, va, Concat q' r2) |q va q'. (q, va, q') \<in> fst (trans2LTS r1 v)})
+                    (insert (Concat \<epsilon> r2, r2) ({(Concat q r2, Concat q' r2) |q q'. (q, q') \<in> snd (trans2LTS r1 v)})) (Concat r1 r2) q (Concat \<epsilon> r2)"
+                    apply (induction rule: LTS_is_reachable.cases)
+                    subgoal for \<Delta> \<Delta>' qa by auto
+                    subgoal for qa q'' \<Delta>' \<Delta> l q' apply auto apply (metis LTS_Step1 insertI1) using c1 by force
+                    subgoal for a qa \<Delta> \<Delta>' w q'  by auto done 
+      then have c3:"LTS_is_reachable ({(Concat q r2, va, Concat q' r2) |q va q'. (q, va, q') \<in> fst (trans2LTS r1 v)} \<union> fst (trans2LTS r2 v))
+                    (insert (Concat \<epsilon> r2, r2) ({(Concat q r2, Concat q' r2) |q q'. (q, q') \<in> snd (trans2LTS r1 v)})  \<union> snd (trans2LTS r2 v))
+            (Concat r1 r2) q (Concat \<epsilon> r2)" using subLTSlemma by fastforce
+      have c4:"LTS_is_reachable ({(Concat q r2, va, Concat q' r2) |q va q'. (q, va, q') \<in> fst (trans2LTS r1 v)} \<union> fst (trans2LTS r2 v))
+               (insert (Concat \<epsilon> r2, r2) ({(Concat q r2, Concat q' r2) |q q'. (q, q') \<in> snd (trans2LTS r1 v)})  \<union> snd (trans2LTS r2 v)) (Concat \<epsilon> r2) [] r2"
+        by (smt (z3) LTS_Empty LTS_Step1 UnI2 Un_commute insert_iff)
+      have c5:"LTS_is_reachable ({(Concat q r2, va, Concat q' r2) |q va q'. (q, va, q') \<in> fst (trans2LTS r1 v)} \<union> fst (trans2LTS r2 v))
+               (insert (Concat \<epsilon> r2, r2) ({(Concat q r2, Concat q' r2) |q q'. (q, q') \<in> snd (trans2LTS r1 v)})  \<union> snd (trans2LTS r2 v)) r2 p \<epsilon>"
+        using a4 by (smt (z3) Un_commute subLTSlemma)
+      have "LTS_is_reachable ({(Concat q r2, va, Concat q' r2) |q va q'. (q, va, q') \<in> fst (trans2LTS r1 v)} \<union> fst (trans2LTS r2 v))
+               (insert (Concat \<epsilon> r2, r2) ({(Concat q r2, Concat q' r2) |q q'. (q, q') \<in> snd (trans2LTS r1 v)})  \<union> snd (trans2LTS r2 v)) (Concat r1 r2) (q @ p) \<epsilon>" using c3 c4 c5 
+        by (smt (z3) LTS_Step1 Un_insert_left insertI1 joinLTSlemma)
       thus ?thesis by auto
     qed
   qed
   subgoal for x 
   proof -
-    assume a1:"sem_reg r1 v = {w. LTS_is_reachable (trans2LTS r1 v) r1 w \<epsilon>}"
-    assume a2:"sem_reg r2 v = {w. LTS_is_reachable (trans2LTS r2 v) r2 w \<epsilon>}"
-    assume a3:"LTS_is_reachable
-     ({(Concat q r2, va, Concat q' r2) |q va q'. (q, va, q') ∈ fst (trans2LTS r1 v)} ∪ fst (trans2LTS r2 v),
-      insert (Concat ε r2, r2) ({(Concat q r2, Concat q' r2) |q q'. (q, q') ∈ snd (trans2LTS r1 v)} ∪ snd (trans2LTS r2 v)))
-     (Concat r1 r2) x ε"
-    show  "∃q p. x = q @ p ∧ LTS_is_reachable (trans2LTS r1 v) r1 q ε ∧ LTS_is_reachable (trans2LTS r2 v) r2 p ε"
-    proof -
-      have c1:"∃q p. x = q @ p \<and> 
-            LTS_is_reachable ({(Concat q r2, va, Concat q' r2) |q va q'. (q, va, q') ∈ fst (trans2LTS r1 v)},
-            {(Concat q r2, Concat q' r2) |q q'. (q, q') ∈ snd (trans2LTS r1 v)}) (Concat r1 r2) q (Concat ε r2) \<and> 
-            LTS_is_reachable (trans2LTS r2 v) r2 p ε"
-        sorry
-      show ?thesis using c1 apply auto sorry
-    qed
+    assume a1:"sem_reg r1 v = {w. LTS_is_reachable (fst (trans2LTS r1 v)) (snd (trans2LTS r1 v)) r1 w \<epsilon>}"
+    assume a2:"sem_reg r2 v = {w. LTS_is_reachable (fst (trans2LTS r2 v)) (snd (trans2LTS r2 v)) r2 w \<epsilon>}"
+    assume a3:"LTS_is_reachable ({(Concat q r2, va, Concat q' r2) |q va q'. (q, va, q') \<in> fst (trans2LTS r1 v)} \<union> fst (trans2LTS r2 v))
+     (insert (Concat \<epsilon> r2, r2) ({(Concat q r2, Concat q' r2) |q q'. (q, q') \<in> snd (trans2LTS r1 v)} \<union> snd (trans2LTS r2 v))) (Concat r1 r2) x \<epsilon>"
+    show  "\<exists>q p. x = q @ p \<and> LTS_is_reachable (fst (trans2LTS r1 v)) (snd (trans2LTS r1 v)) r1 q \<epsilon> \<and> LTS_is_reachable (fst (trans2LTS r2 v)) (snd (trans2LTS r2 v)) r2 p \<epsilon>"
+      sorry
   qed
   done
 next
@@ -369,51 +291,65 @@ next
     apply auto
     subgoal for q p
     proof -
-      assume a1:"sem_reg r v = {w. LTS_is_reachable (trans2LTS r v) r w \<epsilon>}"
-      assume a2:"LTS_is_reachable (trans2LTS r v) r q \<epsilon>"
-      assume a3:"p \<in> star {w. LTS_is_reachable (trans2LTS r v) r w \<epsilon>}"
-      show "LTS_is_reachable ({(Concat (Concat q (Star r)) (Star r), va, Concat (Concat q' (Star r)) (Star r)) |q va q'. (q, va, q') ∈ fst (trans2LTS r v)} ∪
-            {(Concat q (Star r), va, Concat q' (Star r)) |q va q'. (q, va, q') ∈ fst (trans2LTS r v)}, insert (Plus r, Concat (Concat r (Star r)) (Star r))  (insert (Concat (Concat ε (Star r)) (Star r), Concat (Star r) (Star r)) (insert (Concat (Star r) (Star r), ε) (insert (Concat (Star r) (Star r), Concat r (Star r))
-            (insert (Concat ε (Star r), Concat (Star r) (Star r)) ({(Concat (Concat q (Star r)) (Star r), Concat (Concat q' (Star r)) (Star r)) |q q'. (q, q') ∈ snd (trans2LTS r v)} ∪
-            {(Concat q (Star r), Concat q' (Star r)) |q q'. (q, q') ∈ snd (trans2LTS r v)}))))))
-            (Plus r) (q @ p) ε"
+      assume a1:"sem_reg r v = {w. LTS_is_reachable (fst (trans2LTS r v)) (snd (trans2LTS r v)) r w \<epsilon>}"
+      assume a2:"LTS_is_reachable (fst (trans2LTS r v)) (snd (trans2LTS r v)) r q \<epsilon>"
+      assume a3:"p \<in> star {w. LTS_is_reachable (fst (trans2LTS r v)) (snd (trans2LTS r v)) r w \<epsilon>}"
+      show "LTS_is_reachable ({(Concat (Concat q (Star r)) (Star r), va, Concat (Concat q' (Star r)) (Star r)) |q va q'. (q, va, q') \<in> fst (trans2LTS r v)} \<union>
+           {(Concat q (Star r), va, Concat q' (Star r)) |q va q'. (q, va, q') \<in> fst (trans2LTS r v)})
+           (insert (Plus r, Concat (Concat r (Star r)) (Star r)) (insert (Concat (Concat \<epsilon> (Star r)) (Star r), Concat (Star r) (Star r))
+           (insert (Concat (Star r) (Star r), \<epsilon>) (insert (Concat (Star r) (Star r), Concat r (Star r)) (insert (Concat \<epsilon> (Star r), Concat (Star r) (Star r))
+           ({(Concat (Concat q (Star r)) (Star r), Concat (Concat q' (Star r)) (Star r)) |q q'. (q, q') \<in> snd (trans2LTS r v)} \<union>
+           {(Concat q (Star r), Concat q' (Star r)) |q q'. (q, q') \<in> snd (trans2LTS r v)}))))))
+            (Plus r) (q @ p) \<epsilon>"
       proof -
-          have c1:"LTS_is_reachable ({(Concat (Concat q (Star r)) (Star r), va, Concat (Concat q' (Star r)) (Star r)) |q va q'. (q, va, q') ∈ fst (trans2LTS r v)} ∪
-                  {(Concat q (Star r), va, Concat q' (Star r)) |q va q'. (q, va, q') ∈ fst (trans2LTS r v)}, insert (Plus r, Concat (Concat r (Star r)) (Star r))  (insert (Concat (Concat ε (Star r)) (Star r), Concat (Star r) (Star r)) (insert (Concat (Star r) (Star r), ε) (insert (Concat (Star r) (Star r), Concat r (Star r))
-                  (insert (Concat ε (Star r), Concat (Star r) (Star r)) ({(Concat (Concat q (Star r)) (Star r), Concat (Concat q' (Star r)) (Star r)) |q q'. (q, q') ∈ snd (trans2LTS r v)} ∪
-                  {(Concat q (Star r), Concat q' (Star r)) |q q'. (q, q') ∈ snd (trans2LTS r v)}))))))
-                 (Plus r) [] (Concat (Concat r (Star r)) (Star r))"
-            by (smt (verit) LTS_Empty LTS_Step1 insertI1 snd_eqD)
-          have e1:"LTS_is_reachable ({(Concat (Concat q (Star r)) (Star r), va, Concat (Concat q' (Star r)) (Star r)) |q va q'. (q, va, q') ∈ fst (trans2LTS r v)},{(Concat (Concat q (Star r)) (Star r), Concat (Concat q' (Star r)) (Star r)) |q q'. (q, q') ∈ snd (trans2LTS r v)})
+          have c1:"LTS_is_reachable ({(Concat (Concat q (Star r)) (Star r), va, Concat (Concat q' (Star r)) (Star r)) |q va q'. (q, va, q') \<in> fst (trans2LTS r v)} \<union>
+                   {(Concat q (Star r), va, Concat q' (Star r)) |q va q'. (q, va, q') \<in> fst (trans2LTS r v)})
+                   (insert (Plus r, Concat (Concat r (Star r)) (Star r)) (insert (Concat (Concat \<epsilon> (Star r)) (Star r), Concat (Star r) (Star r))
+                   (insert (Concat (Star r) (Star r), \<epsilon>) (insert (Concat (Star r) (Star r), Concat r (Star r)) (insert (Concat \<epsilon> (Star r), Concat (Star r) (Star r))
+                   ({(Concat (Concat q (Star r)) (Star r), Concat (Concat q' (Star r)) (Star r)) |q q'. (q, q') \<in> snd (trans2LTS r v)} \<union>
+                   {(Concat q (Star r), Concat q' (Star r)) |q q'. (q, q') \<in> snd (trans2LTS r v)}))))))
+                   (Plus r) [] (Concat (Concat r (Star r)) (Star r))"
+            by (smt (z3) LTS_Empty LTS_Step1 insertI1)
+          have e1:"LTS_is_reachable ({(Concat (Concat q (Star r)) (Star r), va, Concat (Concat q' (Star r)) (Star r)) |q va q'. (q, va, q') \<in> fst (trans2LTS r v)}) ({(Concat (Concat q (Star r)) (Star r), Concat (Concat q' (Star r)) (Star r)) |q q'. (q, q') \<in> snd (trans2LTS r v)})
                   (Concat (Concat r (Star r)) (Star r)) q (Concat (Concat \<epsilon> (Star r)) (Star r))"
             using a2 by (rule DeltLTSlemma1)
-          have c2:"LTS_is_reachable ({(Concat (Concat q (Star r)) (Star r), va, Concat (Concat q' (Star r)) (Star r)) |q va q'. (q, va, q') ∈ fst (trans2LTS r v)} ∪
-                  {(Concat q (Star r), va, Concat q' (Star r)) |q va q'. (q, va, q') ∈ fst (trans2LTS r v)}, insert (Plus r, Concat (Concat r (Star r)) (Star r))  (insert (Concat (Concat ε (Star r)) (Star r), Concat (Star r) (Star r)) (insert (Concat (Star r) (Star r), ε) (insert (Concat (Star r) (Star r), Concat r (Star r))
-                  (insert (Concat ε (Star r), Concat (Star r) (Star r)) ({(Concat (Concat q (Star r)) (Star r), Concat (Concat q' (Star r)) (Star r)) |q q'. (q, q') ∈ snd (trans2LTS r v)} ∪
-                  {(Concat q (Star r), Concat q' (Star r)) |q q'. (q, q') ∈ snd (trans2LTS r v)}))))))
+          have c2:"LTS_is_reachable ({(Concat (Concat q (Star r)) (Star r), va, Concat (Concat q' (Star r)) (Star r)) |q va q'. (q, va, q') \<in> fst (trans2LTS r v)} \<union>
+                   {(Concat q (Star r), va, Concat q' (Star r)) |q va q'. (q, va, q') \<in> fst (trans2LTS r v)})
+                   (insert (Plus r, Concat (Concat r (Star r)) (Star r)) (insert (Concat (Concat \<epsilon> (Star r)) (Star r), Concat (Star r) (Star r))
+                   (insert (Concat (Star r) (Star r), \<epsilon>) (insert (Concat (Star r) (Star r), Concat r (Star r)) (insert (Concat \<epsilon> (Star r), Concat (Star r) (Star r))
+                   ({(Concat (Concat q (Star r)) (Star r), Concat (Concat q' (Star r)) (Star r)) |q q'. (q, q') \<in> snd (trans2LTS r v)} \<union>
+                   {(Concat q (Star r), Concat q' (Star r)) |q q'. (q, q') \<in> snd (trans2LTS r v)}))))))
                   (Concat (Concat r (Star r)) (Star r)) q (Concat (Concat \<epsilon> (Star r)) (Star r))"
-            using e1   by (metis (no_types, lifting) Un_insert_right fst_eqD snd_eqD subLTSlemma)
-          have 1:"LTS_is_reachable ({(Concat (Concat q (Star r)) (Star r), va, Concat (Concat q' (Star r)) (Star r)) |q va q'. (q, va, q') ∈ fst (trans2LTS r v)} ∪
-                  {(Concat q (Star r), va, Concat q' (Star r)) |q va q'. (q, va, q') ∈ fst (trans2LTS r v)}, insert (Plus r, Concat (Concat r (Star r)) (Star r)) (insert (Concat (Concat ε (Star r)) (Star r), Concat (Star r) (Star r))
-                  (insert (Concat (Star r) (Star r), ε) (insert (Concat (Star r) (Star r), Concat r (Star r)) (insert (Concat ε (Star r), Concat (Star r) (Star r)) ({(Concat (Concat q (Star r)) (Star r), Concat (Concat q' (Star r)) (Star r)) |q q'. (q, q') ∈ snd (trans2LTS r v)} ∪
-                  {(Concat q (Star r), Concat q' (Star r)) |q q'. (q, q') ∈ snd (trans2LTS r v)}))))))
+            using e1 by (smt (z3) Un_insert_right subLTSlemma) 
+          have 1:"LTS_is_reachable ({(Concat (Concat q (Star r)) (Star r), va, Concat (Concat q' (Star r)) (Star r)) |q va q'. (q, va, q') \<in> fst (trans2LTS r v)} \<union>
+                   {(Concat q (Star r), va, Concat q' (Star r)) |q va q'. (q, va, q') \<in> fst (trans2LTS r v)})
+                   (insert (Plus r, Concat (Concat r (Star r)) (Star r)) (insert (Concat (Concat \<epsilon> (Star r)) (Star r), Concat (Star r) (Star r))
+                   (insert (Concat (Star r) (Star r), \<epsilon>) (insert (Concat (Star r) (Star r), Concat r (Star r)) (insert (Concat \<epsilon> (Star r), Concat (Star r) (Star r))
+                   ({(Concat (Concat q (Star r)) (Star r), Concat (Concat q' (Star r)) (Star r)) |q q'. (q, q') \<in> snd (trans2LTS r v)} \<union>
+                   {(Concat q (Star r), Concat q' (Star r)) |q q'. (q, q') \<in> snd (trans2LTS r v)}))))))
                   (Plus r) q (Concat (Concat \<epsilon> (Star r)) (Star r))"
             using c1 c2 joinLTSlemma by fastforce
-          have c3:"LTS_is_reachable ({(Concat (Concat q (Star r)) (Star r), va, Concat (Concat q' (Star r)) (Star r)) |q va q'. (q, va, q') ∈ fst (trans2LTS r v)} ∪
-                  {(Concat q (Star r), va, Concat q' (Star r)) |q va q'. (q, va, q') ∈ fst (trans2LTS r v)}, insert (Plus r, Concat (Concat r (Star r)) (Star r)) (insert (Concat (Concat ε (Star r)) (Star r), Concat (Star r) (Star r))
-                  (insert (Concat (Star r) (Star r), ε) (insert (Concat (Star r) (Star r), Concat r (Star r)) (insert (Concat ε (Star r), Concat (Star r) (Star r)) ({(Concat (Concat q (Star r)) (Star r), Concat (Concat q' (Star r)) (Star r)) |q q'. (q, q') ∈ snd (trans2LTS r v)} ∪
-                  {(Concat q (Star r), Concat q' (Star r)) |q q'. (q, q') ∈ snd (trans2LTS r v)}))))))
+          have c3:"LTS_is_reachable ({(Concat (Concat q (Star r)) (Star r), va, Concat (Concat q' (Star r)) (Star r)) |q va q'. (q, va, q') \<in> fst (trans2LTS r v)} \<union>
+                   {(Concat q (Star r), va, Concat q' (Star r)) |q va q'. (q, va, q') \<in> fst (trans2LTS r v)})
+                   (insert (Plus r, Concat (Concat r (Star r)) (Star r)) (insert (Concat (Concat \<epsilon> (Star r)) (Star r), Concat (Star r) (Star r))
+                   (insert (Concat (Star r) (Star r), \<epsilon>) (insert (Concat (Star r) (Star r), Concat r (Star r)) (insert (Concat \<epsilon> (Star r), Concat (Star r) (Star r))
+                   ({(Concat (Concat q (Star r)) (Star r), Concat (Concat q' (Star r)) (Star r)) |q q'. (q, q') \<in> snd (trans2LTS r v)} \<union>
+                   {(Concat q (Star r), Concat q' (Star r)) |q q'. (q, q') \<in> snd (trans2LTS r v)}))))))
                   (Concat (Concat \<epsilon> (Star r)) (Star r)) []  (Concat (Star r) (Star r))" 
-            by (smt (z3) LTS_Empty LTS_Step1 insertI1 insert_commute snd_conv)
-          have 2:"LTS_is_reachable ({(Concat (Concat q (Star r)) (Star r), va, Concat (Concat q' (Star r)) (Star r)) |q va q'. (q, va, q') ∈ fst (trans2LTS r v)} ∪
-                  {(Concat q (Star r), va, Concat q' (Star r)) |q va q'. (q, va, q') ∈ fst (trans2LTS r v)}, insert (Plus r, Concat (Concat r (Star r)) (Star r)) (insert (Concat (Concat ε (Star r)) (Star r), Concat (Star r) (Star r))
-                  (insert (Concat (Star r) (Star r), ε) (insert (Concat (Star r) (Star r), Concat r (Star r)) (insert (Concat ε (Star r), Concat (Star r) (Star r)) ({(Concat (Concat q (Star r)) (Star r), Concat (Concat q' (Star r)) (Star r)) |q q'. (q, q') ∈ snd (trans2LTS r v)} ∪
-                  {(Concat q (Star r), Concat q' (Star r)) |q q'. (q, q') ∈ snd (trans2LTS r v)}))))))
+            by (smt (verit, best) LTS_Empty LTS_Step1 insert_iff)
+          have 2:"LTS_is_reachable ({(Concat (Concat q (Star r)) (Star r), va, Concat (Concat q' (Star r)) (Star r)) |q va q'. (q, va, q') \<in> fst (trans2LTS r v)} \<union>
+                   {(Concat q (Star r), va, Concat q' (Star r)) |q va q'. (q, va, q') \<in> fst (trans2LTS r v)})
+                   (insert (Plus r, Concat (Concat r (Star r)) (Star r)) (insert (Concat (Concat \<epsilon> (Star r)) (Star r), Concat (Star r) (Star r))
+                   (insert (Concat (Star r) (Star r), \<epsilon>) (insert (Concat (Star r) (Star r), Concat r (Star r)) (insert (Concat \<epsilon> (Star r), Concat (Star r) (Star r))
+                   ({(Concat (Concat q (Star r)) (Star r), Concat (Concat q' (Star r)) (Star r)) |q q'. (q, q') \<in> snd (trans2LTS r v)} \<union>
+                   {(Concat q (Star r), Concat q' (Star r)) |q q'. (q, q') \<in> snd (trans2LTS r v)}))))))
                   (Plus r) q  (Concat (Star r) (Star r))" using 1 c3 joinLTSlemma by fastforce
-          have 3:"LTS_is_reachable ({(Concat (Concat q (Star r)) (Star r), va, Concat (Concat q' (Star r)) (Star r)) |q va q'. (q, va, q') ∈ fst (trans2LTS r v)} ∪
-                    {(Concat q (Star r), va, Concat q' (Star r)) |q va q'. (q, va, q') ∈ fst (trans2LTS r v)}, insert (Plus r, Concat (Concat r (Star r)) (Star r)) (insert (Concat (Concat ε (Star r)) (Star r), Concat (Star r) (Star r))
-                    (insert (Concat (Star r) (Star r), ε) (insert (Concat (Star r) (Star r), Concat r (Star r)) (insert (Concat ε (Star r), Concat (Star r) (Star r)) ({(Concat (Concat q (Star r)) (Star r), Concat (Concat q' (Star r)) (Star r)) |q q'. (q, q') ∈ snd (trans2LTS r v)} ∪
-                    {(Concat q (Star r), Concat q' (Star r)) |q q'. (q, q') ∈ snd (trans2LTS r v)}))))))
+          have 3:"LTS_is_reachable ({(Concat (Concat q (Star r)) (Star r), va, Concat (Concat q' (Star r)) (Star r)) |q va q'. (q, va, q') \<in> fst (trans2LTS r v)} \<union>
+                   {(Concat q (Star r), va, Concat q' (Star r)) |q va q'. (q, va, q') \<in> fst (trans2LTS r v)})
+                   (insert (Plus r, Concat (Concat r (Star r)) (Star r)) (insert (Concat (Concat \<epsilon> (Star r)) (Star r), Concat (Star r) (Star r))
+                   (insert (Concat (Star r) (Star r), \<epsilon>) (insert (Concat (Star r) (Star r), Concat r (Star r)) (insert (Concat \<epsilon> (Star r), Concat (Star r) (Star r))
+                   ({(Concat (Concat q (Star r)) (Star r), Concat (Concat q' (Star r)) (Star r)) |q q'. (q, q') \<in> snd (trans2LTS r v)} \<union>
+                   {(Concat q (Star r), Concat q' (Star r)) |q q'. (q, q') \<in> snd (trans2LTS r v)}))))))
                    (Concat (Star r) (Star r)) p \<epsilon>"
                 using a3 proof(induction p)
                   case zero
@@ -422,45 +358,56 @@ next
                 next
                   case (step x y)
                   then show ?case apply auto proof -
-                    assume a1:"LTS_is_reachable (trans2LTS r v) r x \<epsilon>"
-                    assume a2:"y \<in> star {w. LTS_is_reachable (trans2LTS r v) r w \<epsilon>}"
-                    assume a3:"LTS_is_reachable ({(Concat (Concat q (Star r)) (Star r), va, Concat (Concat q' (Star r)) (Star r)) |q va q'. (q, va, q') ∈ fst (trans2LTS r v)} ∪
-                              {(Concat q (Star r), va, Concat q' (Star r)) |q va q'. (q, va, q') ∈ fst (trans2LTS r v)}, insert (Plus r, Concat (Concat r (Star r)) (Star r))
-                              (insert (Concat (Concat ε (Star r)) (Star r), Concat (Star r) (Star r)) (insert (Concat (Star r) (Star r), ε) (insert (Concat (Star r) (Star r), Concat r (Star r)) (insert (Concat ε (Star r), Concat (Star r) (Star r))
-                              ({(Concat (Concat q (Star r)) (Star r), Concat (Concat q' (Star r)) (Star r)) |q q'. (q, q') ∈ snd (trans2LTS r v)} ∪ {(Concat q (Star r), Concat q' (Star r)) |q q'. (q, q') ∈ snd (trans2LTS r v)}))))))
-                              (Concat (Star r) (Star r)) y ε"
-                    have e1:"LTS_is_reachable ({(Concat q (Star r), va, Concat q' (Star r)) |q va q'. (q, va, q') \<in> fst (trans2LTS r v)}, 
-                          {(Concat q (Star r), Concat q' (Star r)) |q q'. (q, q') \<in> snd (trans2LTS r v)}) (Concat r (Star r)) x (Concat \<epsilon> (Star r))"
+                    assume a1:"LTS_is_reachable (fst (trans2LTS r v)) (snd (trans2LTS r v)) r x \<epsilon>"
+                    assume a2:"y \<in> star {w. LTS_is_reachable (fst (trans2LTS r v)) (snd (trans2LTS r v)) r w \<epsilon>}"
+                    assume a3:"LTS_is_reachable ({(Concat (Concat q (Star r)) (Star r), va, Concat (Concat q' (Star r)) (Star r)) |q va q'. (q, va, q') \<in> fst (trans2LTS r v)} \<union>
+                               {(Concat q (Star r), va, Concat q' (Star r)) |q va q'. (q, va, q') \<in> fst (trans2LTS r v)})
+                               (insert (Plus r, Concat (Concat r (Star r)) (Star r)) (insert (Concat (Concat \<epsilon> (Star r)) (Star r), Concat (Star r) (Star r))
+                               (insert (Concat (Star r) (Star r), \<epsilon>) (insert (Concat (Star r) (Star r), Concat r (Star r)) (insert (Concat \<epsilon> (Star r), Concat (Star r) (Star r))
+                               ({(Concat (Concat q (Star r)) (Star r), Concat (Concat q' (Star r)) (Star r)) |q q'. (q, q') \<in> snd (trans2LTS r v)} \<union>
+                                {(Concat q (Star r), Concat q' (Star r)) |q q'. (q, q') \<in> snd (trans2LTS r v)}))))))
+                               (Concat (Star r) (Star r)) y \<epsilon>"
+                    have e1:"LTS_is_reachable ({(Concat q (Star r), va, Concat q' (Star r)) |q va q'. (q, va, q') \<in> fst (trans2LTS r v)}) ({(Concat q (Star r), Concat q' (Star r)) |q q'. (q, q') \<in> snd (trans2LTS r v)}) (Concat r (Star r)) x (Concat \<epsilon> (Star r))"
                       using a1 by(simp add:DeltLTSlemma1)
-                    have e2:"LTS_is_reachable ({(Concat (Concat q (Star r)) (Star r), va, Concat (Concat q' (Star r)) (Star r)) |q va q'. (q, va, q') ∈ fst (trans2LTS r v)} ∪
-                              {(Concat q (Star r), va, Concat q' (Star r)) |q va q'. (q, va, q') ∈ fst (trans2LTS r v)}, insert (Plus r, Concat (Concat r (Star r)) (Star r))
-                              (insert (Concat (Concat ε (Star r)) (Star r), Concat (Star r) (Star r)) (insert (Concat (Star r) (Star r), ε) (insert (Concat (Star r) (Star r), Concat r (Star r)) (insert (Concat ε (Star r), Concat (Star r) (Star r))
-                              ({(Concat (Concat q (Star r)) (Star r), Concat (Concat q' (Star r)) (Star r)) |q q'. (q, q') ∈ snd (trans2LTS r v)} ∪ {(Concat q (Star r), Concat q' (Star r)) |q q'. (q, q') ∈ snd (trans2LTS r v)}))))))
+                    have e2:"LTS_is_reachable ({(Concat (Concat q (Star r)) (Star r), va, Concat (Concat q' (Star r)) (Star r)) |q va q'. (q, va, q') \<in> fst (trans2LTS r v)} \<union>
+                               {(Concat q (Star r), va, Concat q' (Star r)) |q va q'. (q, va, q') \<in> fst (trans2LTS r v)})
+                               (insert (Plus r, Concat (Concat r (Star r)) (Star r)) (insert (Concat (Concat \<epsilon> (Star r)) (Star r), Concat (Star r) (Star r))
+                               (insert (Concat (Star r) (Star r), \<epsilon>) (insert (Concat (Star r) (Star r), Concat r (Star r)) (insert (Concat \<epsilon> (Star r), Concat (Star r) (Star r))
+                               ({(Concat (Concat q (Star r)) (Star r), Concat (Concat q' (Star r)) (Star r)) |q q'. (q, q') \<in> snd (trans2LTS r v)} \<union>
+                                {(Concat q (Star r), Concat q' (Star r)) |q q'. (q, q') \<in> snd (trans2LTS r v)}))))))
                               (Concat (Star r) (Star r)) [] (Concat r (Star r))"
-                      by (smt (z3) LTS_Empty LTS_Step1 insertI1 insert_commute snd_conv)
-                   have c1:"LTS_is_reachable ({(Concat (Concat q (Star r)) (Star r), va, Concat (Concat q' (Star r)) (Star r)) |q va q'. (q, va, q') ∈ fst (trans2LTS r v)} ∪
-                              {(Concat q (Star r), va, Concat q' (Star r)) |q va q'. (q, va, q') ∈ fst (trans2LTS r v)}, insert (Plus r, Concat (Concat r (Star r)) (Star r))
-                              (insert (Concat (Concat ε (Star r)) (Star r), Concat (Star r) (Star r)) (insert (Concat (Star r) (Star r), ε) (insert (Concat (Star r) (Star r), Concat r (Star r)) (insert (Concat ε (Star r), Concat (Star r) (Star r))
-                              ({(Concat (Concat q (Star r)) (Star r), Concat (Concat q' (Star r)) (Star r)) |q q'. (q, q') ∈ snd (trans2LTS r v)} ∪ {(Concat q (Star r), Concat q' (Star r)) |q q'. (q, q') ∈ snd (trans2LTS r v)}))))))
+                      by (smt (verit, best) LTS_Empty LTS_Step1 insertI1 insertI2)
+                   have c1:"LTS_is_reachable ({(Concat (Concat q (Star r)) (Star r), va, Concat (Concat q' (Star r)) (Star r)) |q va q'. (q, va, q') \<in> fst (trans2LTS r v)} \<union>
+                               {(Concat q (Star r), va, Concat q' (Star r)) |q va q'. (q, va, q') \<in> fst (trans2LTS r v)})
+                               (insert (Plus r, Concat (Concat r (Star r)) (Star r)) (insert (Concat (Concat \<epsilon> (Star r)) (Star r), Concat (Star r) (Star r))
+                               (insert (Concat (Star r) (Star r), \<epsilon>) (insert (Concat (Star r) (Star r), Concat r (Star r)) (insert (Concat \<epsilon> (Star r), Concat (Star r) (Star r))
+                               ({(Concat (Concat q (Star r)) (Star r), Concat (Concat q' (Star r)) (Star r)) |q q'. (q, q') \<in> snd (trans2LTS r v)} \<union>
+                                {(Concat q (Star r), Concat q' (Star r)) |q q'. (q, q') \<in> snd (trans2LTS r v)}))))))
                              (Concat r (Star r)) x (Concat \<epsilon> (Star r))"
-                     using e1   by (smt (z3) Un_left_commute fst_conv inf_sup_aci(5) insert_def snd_conv subLTSlemma)
-                    have e3:"LTS_is_reachable ({(Concat (Concat q (Star r)) (Star r), va, Concat (Concat q' (Star r)) (Star r)) |q va q'. (q, va, q') ∈ fst (trans2LTS r v)} ∪
-                              {(Concat q (Star r), va, Concat q' (Star r)) |q va q'. (q, va, q') ∈ fst (trans2LTS r v)}, insert (Plus r, Concat (Concat r (Star r)) (Star r))
-                              (insert (Concat (Concat ε (Star r)) (Star r), Concat (Star r) (Star r)) (insert (Concat (Star r) (Star r), ε) (insert (Concat (Star r) (Star r), Concat r (Star r)) (insert (Concat ε (Star r), Concat (Star r) (Star r))
-                              ({(Concat (Concat q (Star r)) (Star r), Concat (Concat q' (Star r)) (Star r)) |q q'. (q, q') ∈ snd (trans2LTS r v)} ∪ {(Concat q (Star r), Concat q' (Star r)) |q q'. (q, q') ∈ snd (trans2LTS r v)}))))))
-                              (Concat (Star r) (Star r)) x (Concat \<epsilon> (Star r))"
+                     using e1 by (smt (z3) Un_insert_left subLTSlemma sup_commute) 
+                    have e3:"LTS_is_reachable ({(Concat (Concat q (Star r)) (Star r), va, Concat (Concat q' (Star r)) (Star r)) |q va q'. (q, va, q') \<in> fst (trans2LTS r v)} \<union>
+                               {(Concat q (Star r), va, Concat q' (Star r)) |q va q'. (q, va, q') \<in> fst (trans2LTS r v)})
+                               (insert (Plus r, Concat (Concat r (Star r)) (Star r)) (insert (Concat (Concat \<epsilon> (Star r)) (Star r), Concat (Star r) (Star r))
+                               (insert (Concat (Star r) (Star r), \<epsilon>) (insert (Concat (Star r) (Star r), Concat r (Star r)) (insert (Concat \<epsilon> (Star r), Concat (Star r) (Star r))
+                               ({(Concat (Concat q (Star r)) (Star r), Concat (Concat q' (Star r)) (Star r)) |q q'. (q, q') \<in> snd (trans2LTS r v)} \<union>
+                                {(Concat q (Star r), Concat q' (Star r)) |q q'. (q, q') \<in> snd (trans2LTS r v)}))))))
+                                  (Concat (Star r) (Star r)) x (Concat \<epsilon> (Star r))"
                       using e2 c1 joinLTSlemma by fastforce
-                    have c2:"LTS_is_reachable ({(Concat (Concat q (Star r)) (Star r), va, Concat (Concat q' (Star r)) (Star r)) |q va q'. (q, va, q') ∈ fst (trans2LTS r v)} ∪
-                              {(Concat q (Star r), va, Concat q' (Star r)) |q va q'. (q, va, q') ∈ fst (trans2LTS r v)}, insert (Plus r, Concat (Concat r (Star r)) (Star r))
-                              (insert (Concat (Concat ε (Star r)) (Star r), Concat (Star r) (Star r)) (insert (Concat (Star r) (Star r), ε) (insert (Concat (Star r) (Star r), Concat r (Star r)) (insert (Concat ε (Star r), Concat (Star r) (Star r))
-                              ({(Concat (Concat q (Star r)) (Star r), Concat (Concat q' (Star r)) (Star r)) |q q'. (q, q') ∈ snd (trans2LTS r v)} ∪ {(Concat q (Star r), Concat q' (Star r)) |q q'. (q, q') ∈ snd (trans2LTS r v)}))))))
-                              (Concat \<epsilon> (Star r)) [] (Concat (Star r) (Star r))"
+                    have c2:"LTS_is_reachable ({(Concat (Concat q (Star r)) (Star r), va, Concat (Concat q' (Star r)) (Star r)) |q va q'. (q, va, q') \<in> fst (trans2LTS r v)} \<union>
+                               {(Concat q (Star r), va, Concat q' (Star r)) |q va q'. (q, va, q') \<in> fst (trans2LTS r v)})
+                               (insert (Plus r, Concat (Concat r (Star r)) (Star r)) (insert (Concat (Concat \<epsilon> (Star r)) (Star r), Concat (Star r) (Star r))
+                               (insert (Concat (Star r) (Star r), \<epsilon>) (insert (Concat (Star r) (Star r), Concat r (Star r)) (insert (Concat \<epsilon> (Star r), Concat (Star r) (Star r))
+                               ({(Concat (Concat q (Star r)) (Star r), Concat (Concat q' (Star r)) (Star r)) |q q'. (q, q') \<in> snd (trans2LTS r v)} \<union>
+                                {(Concat q (Star r), Concat q' (Star r)) |q q'. (q, q') \<in> snd (trans2LTS r v)}))))))
+                              (Concat \<epsilon> (Star r)) [] (Concat (Star r) (Star r))" 
                       by (smt (verit, ccfv_threshold) LTS_Empty LTS_Step1 insertI1 insert_commute snd_conv)
-                    have e4:"LTS_is_reachable ({(Concat (Concat q (Star r)) (Star r), va, Concat (Concat q' (Star r)) (Star r)) |q va q'. (q, va, q') ∈ fst (trans2LTS r v)} ∪
-                              {(Concat q (Star r), va, Concat q' (Star r)) |q va q'. (q, va, q') ∈ fst (trans2LTS r v)}, insert (Plus r, Concat (Concat r (Star r)) (Star r))
-                              (insert (Concat (Concat ε (Star r)) (Star r), Concat (Star r) (Star r)) (insert (Concat (Star r) (Star r), ε) (insert (Concat (Star r) (Star r), Concat r (Star r)) (insert (Concat ε (Star r), Concat (Star r) (Star r))
-                              ({(Concat (Concat q (Star r)) (Star r), Concat (Concat q' (Star r)) (Star r)) |q q'. (q, q') ∈ snd (trans2LTS r v)} ∪ {(Concat q (Star r), Concat q' (Star r)) |q q'. (q, q') ∈ snd (trans2LTS r v)}))))))
-                              (Concat (Star r) (Star r)) x (Concat (Star r) (Star r))"using e3 c2 joinLTSlemma by fastforce
+                    have e4:"LTS_is_reachable ({(Concat (Concat q (Star r)) (Star r), va, Concat (Concat q' (Star r)) (Star r)) |q va q'. (q, va, q') \<in> fst (trans2LTS r v)} \<union>
+                               {(Concat q (Star r), va, Concat q' (Star r)) |q va q'. (q, va, q') \<in> fst (trans2LTS r v)})
+                               (insert (Plus r, Concat (Concat r (Star r)) (Star r)) (insert (Concat (Concat \<epsilon> (Star r)) (Star r), Concat (Star r) (Star r))
+                               (insert (Concat (Star r) (Star r), \<epsilon>) (insert (Concat (Star r) (Star r), Concat r (Star r)) (insert (Concat \<epsilon> (Star r), Concat (Star r) (Star r))
+                               ({(Concat (Concat q (Star r)) (Star r), Concat (Concat q' (Star r)) (Star r)) |q q'. (q, q') \<in> snd (trans2LTS r v)} \<union>
+                                {(Concat q (Star r), Concat q' (Star r)) |q q'. (q, q') \<in> snd (trans2LTS r v)}))))))
+                              (Concat (Star r) (Star r)) x (Concat (Star r) (Star r))" using e3 c2 joinLTSlemma by (smt (z3) append_Nil2)
                     thus ?thesis using e4 a3 joinLTSlemma by fastforce
                   qed
                 qed
@@ -469,13 +416,14 @@ next
      qed
     subgoal for x 
     proof -
-      assume "sem_reg r v = {w. LTS_is_reachable (trans2LTS r v) r w \<epsilon>}"
-      assume "LTS_is_reachable ({(Concat (Concat q (Star r)) (Star r), va, Concat (Concat q' (Star r)) (Star r)) |q va q'. (q, va, q') ∈ fst (trans2LTS r v)} ∪
-              {(Concat q (Star r), va, Concat q' (Star r)) |q va q'. (q, va, q') ∈ fst (trans2LTS r v)}, insert (Plus r, Concat (Concat r (Star r)) (Star r)) (insert (Concat (Concat ε (Star r)) (Star r), Concat (Star r) (Star r))
-              (insert (Concat (Star r) (Star r), ε) (insert (Concat (Star r) (Star r), Concat r (Star r)) (insert (Concat ε (Star r), Concat (Star r) (Star r)) ({(Concat (Concat q (Star r)) (Star r), Concat (Concat q' (Star r)) (Star r)) |q q'. (q, q') ∈ snd (trans2LTS r v)} ∪
-              {(Concat q (Star r), Concat q' (Star r)) |q q'. (q, q') ∈ snd (trans2LTS r v)}))))))
-              (Plus r) x ε"
-      show "\<exists>q p. x = q @ p \<and> LTS_is_reachable (trans2LTS r v) r q \<epsilon> \<and> p \<in> star {w. LTS_is_reachable (trans2LTS r v) r w \<epsilon>}"  
+      assume "sem_reg r v = {w. LTS_is_reachable (fst (trans2LTS r v)) (snd (trans2LTS r v)) r w \<epsilon>}"
+      assume "LTS_is_reachable ({(Concat (Concat q (Star r)) (Star r), va, Concat (Concat q' (Star r)) (Star r)) |q va q'. (q, va, q') \<in> fst (trans2LTS r v)} \<union>
+             {(Concat q (Star r), va, Concat q' (Star r)) |q va q'. (q, va, q') \<in> fst (trans2LTS r v)}) (insert (Plus r, Concat (Concat r (Star r)) (Star r))
+             (insert (Concat (Concat \<epsilon> (Star r)) (Star r), Concat (Star r) (Star r)) (insert (Concat (Star r) (Star r), \<epsilon>) (insert (Concat (Star r) (Star r), Concat r (Star r))
+             (insert (Concat \<epsilon> (Star r), Concat (Star r) (Star r)) ({(Concat (Concat q (Star r)) (Star r), Concat (Concat q' (Star r)) (Star r)) |q q'. (q, q') \<in> snd (trans2LTS r v)} \<union>
+             {(Concat q (Star r), Concat q' (Star r)) |q q'. (q, q') \<in> snd (trans2LTS r v)}))))))
+             (Plus r) x \<epsilon>"
+      show "\<exists>q p. x = q @ p \<and> LTS_is_reachable (fst (trans2LTS r v)) (snd (trans2LTS r v)) r q \<epsilon> \<and> p \<in> star {w. LTS_is_reachable (fst (trans2LTS r v)) (snd (trans2LTS r v)) r w \<epsilon>}"  
         sorry 
     qed
     done
@@ -486,67 +434,65 @@ next
      apply auto 
     subgoal for x 
     proof -
-      assume a1:"sem_reg r v = {w. LTS_is_reachable (trans2LTS r v) r w \<epsilon>}"
-      assume a2:"x \<in> star {w. LTS_is_reachable (trans2LTS r v) r w \<epsilon>}"
-      show "LTS_is_reachable
-     ({(Concat q (Star r), va, Concat q' (Star r)) |q va q'. (q, va, q') \<in> fst (trans2LTS r v)},
-      insert (Star r, \<epsilon>) (insert (Star r, Concat r (Star r)) (insert (Concat \<epsilon> (Star r), Star r) {(Concat q (Star r), Concat q' (Star r)) |q q'. (q, q') \<in> snd (trans2LTS r v)})))
-     (Star r) x \<epsilon>" 
-        using a2 proof (induction x)
+      assume a1:"sem_reg r v = {w. LTS_is_reachable (fst (trans2LTS r v)) (snd (trans2LTS r v)) r w \<epsilon>}"
+      assume a2:"x \<in> star {w. LTS_is_reachable (fst (trans2LTS r v)) (snd (trans2LTS r v)) r w \<epsilon>}"
+      show "LTS_is_reachable {(Concat q (Star r), va, Concat q' (Star r)) |q va q'. (q, va, q') \<in> fst (trans2LTS r v)}
+           (insert (Star r, \<epsilon>) (insert (Star r, Concat r (Star r)) (insert (Concat \<epsilon> (Star r), Star r) {(Concat q (Star r), Concat q' (Star r)) |q q'. (q, q') \<in> snd (trans2LTS r v)})))
+           (Star r) x \<epsilon>" using a2 
+      proof (induction x)
         case zero
         then show ?case
-          by (metis (no_types, lifting) LTS_Empty LTS_Step1 insertI1 snd_conv)
+          by (smt (verit, best) LTS_Empty LTS_Step1 insertI1)
       next
         case (step x y)
         then show ?case apply auto 
         proof -
-          assume a1:"LTS_is_reachable (trans2LTS r v) r x \<epsilon>"
-          assume a2:"y \<in> star {w. LTS_is_reachable (trans2LTS r v) r w \<epsilon>}"
-          assume a3:"LTS_is_reachable ({(Concat q (Star r), va, Concat q' (Star r)) |q va q'. (q, va, q') \<in> fst (trans2LTS r v)},
-                    insert (Star r, \<epsilon>) (insert (Star r, Concat r (Star r)) (insert (Concat \<epsilon> (Star r), Star r) {(Concat q (Star r), Concat q' (Star r)) |q q'. (q, q') \<in> snd (trans2LTS r v)})))
-                   (Star r) y \<epsilon>"
-          show "LTS_is_reachable ({(Concat q (Star r), va, Concat q' (Star r)) |q va q'. (q, va, q') \<in> fst (trans2LTS r v)},
-                    insert (Star r, \<epsilon>) (insert (Star r, Concat r (Star r)) (insert (Concat \<epsilon> (Star r), Star r) {(Concat q (Star r), Concat q' (Star r)) |q q'. (q, q') \<in> snd (trans2LTS r v)})))
-                   (Star r) (x @ y) \<epsilon>"
+          assume a1:"LTS_is_reachable (fst (trans2LTS r v)) (snd (trans2LTS r v)) r x \<epsilon>"
+          assume a2:"y \<in> star {w. LTS_is_reachable (fst (trans2LTS r v)) (snd (trans2LTS r v)) r w \<epsilon>}"
+          assume a3:"LTS_is_reachable {(Concat q (Star r), va, Concat q' (Star r)) |q va q'. (q, va, q') \<in> fst (trans2LTS r v)}
+                     (insert (Star r, \<epsilon>) (insert (Star r, Concat r (Star r)) (insert (Concat \<epsilon> (Star r), Star r) {(Concat q (Star r), Concat q' (Star r)) |q q'. (q, q') \<in> snd (trans2LTS r v)})))
+                     (Star r) y \<epsilon>"
+          show "LTS_is_reachable {(Concat q (Star r), va, Concat q' (Star r)) |q va q'. (q, va, q') \<in> fst (trans2LTS r v)}
+                     (insert (Star r, \<epsilon>) (insert (Star r, Concat r (Star r)) (insert (Concat \<epsilon> (Star r), Star r) {(Concat q (Star r), Concat q' (Star r)) |q q'. (q, q') \<in> snd (trans2LTS r v)})))
+                     (Star r) (x @ y) \<epsilon>"
           proof -
-            have c1:"LTS_is_reachable ({(Concat q (Star r), va, Concat q' (Star r)) |q va q'. (q, va, q') \<in> fst (trans2LTS r v)},
-                    insert (Star r, \<epsilon>) (insert (Star r, Concat r (Star r)) (insert (Concat \<epsilon> (Star r), Star r) {(Concat q (Star r), Concat q' (Star r)) |q q'. (q, q') \<in> snd (trans2LTS r v)})))
+            have c1:"LTS_is_reachable {(Concat q (Star r), va, Concat q' (Star r)) |q va q'. (q, va, q') \<in> fst (trans2LTS r v)}
+                     (insert (Star r, \<epsilon>) (insert (Star r, Concat r (Star r)) (insert (Concat \<epsilon> (Star r), Star r) {(Concat q (Star r), Concat q' (Star r)) |q q'. (q, q') \<in> snd (trans2LTS r v)})))
                     (Star r) [] (Concat r (Star r))"
               by (smt (z3) LTS_Empty LTS_Step1 insert_iff snd_conv)
-            have c2:"LTS_is_reachable ({(Concat q (Star r), va, Concat q' (Star r)) |q va q'. (q, va, q') \<in> fst (trans2LTS r v)} , {(Concat q (Star r), Concat q' (Star r)) |q q'. (q, q') \<in> snd (trans2LTS r v)})
+            have c2:"LTS_is_reachable ({(Concat q (Star r), va, Concat q' (Star r)) |q va q'. (q, va, q') \<in> fst (trans2LTS r v)}) ({(Concat q (Star r), Concat q' (Star r)) |q q'. (q, q') \<in> snd (trans2LTS r v)})
                     (Concat r (Star r)) x (Concat \<epsilon> (Star r))"
               using a1 by(simp add:DeltLTSlemma1)
-            have c4:"LTS_is_reachable ({(Concat q (Star r), va, Concat q' (Star r)) |q va q'. (q, va, q') \<in> fst (trans2LTS r v)} \<union> fst (trans2LTS r v),
-                    {(Concat q (Star r), Concat q' (Star r)) |q q'. (q, q') \<in> snd (trans2LTS r v)})
+            have c4:"LTS_is_reachable ({(Concat q (Star r), va, Concat q' (Star r)) |q va q'. (q, va, q') \<in> fst (trans2LTS r v)} \<union> fst (trans2LTS r v))
+                    ({(Concat q (Star r), Concat q' (Star r)) |q q'. (q, q') \<in> snd (trans2LTS r v)})
                     (Concat r (Star r)) x (Concat \<epsilon> (Star r))"
-              using c2 by (smt (verit, best) Collect_cong Collect_disj_eq fst_eqD snd_eqD subLTSlemma)
-            have c5:"LTS_is_reachable ({(Concat q (Star r), va, Concat q' (Star r)) |q va q'. (q, va, q') \<in> fst (trans2LTS r v)} \<union> fst (trans2LTS r v),
-                     (insert (Concat \<epsilon> (Star r), Star r) {(Concat q (Star r), Concat q' (Star r)) |q q'. (q, q') \<in> snd (trans2LTS r v)}))
+              using c2 by (metis (mono_tags, lifting) Collect_cong Collect_disj_eq subLTSlemma)
+            have c5:"LTS_is_reachable ({(Concat q (Star r), va, Concat q' (Star r)) |q va q'. (q, va, q') \<in> fst (trans2LTS r v)} \<union> fst (trans2LTS r v)) 
+                     ((insert (Concat \<epsilon> (Star r), Star r) {(Concat q (Star r), Concat q' (Star r)) |q q'. (q, q') \<in> snd (trans2LTS r v)}))
                      (Concat r (Star r)) x (Concat \<epsilon> (Star r))"
-              using c4 
-              by (smt (verit, best) Collect_cong Collect_disj_eq Un_insert_right c2 fst_eqD snd_eqD subLTSlemma)
-            have c6:"LTS_is_reachable  ({(Concat q (Star r), va, Concat q' (Star r)) |q va q'. (q, va, q') \<in> fst (trans2LTS r v)} \<union> fst (trans2LTS r v),
-                    (insert (Star r, Concat r (Star r)) (insert (Concat \<epsilon> (Star r), Star r) {(Concat q (Star r), Concat q' (Star r)) |q q'. (q, q') \<in> snd (trans2LTS r v)})))
+              using c4 by (smt (verit, best) Collect_cong Collect_disj_eq Un_insert_right c2 fst_eqD snd_eqD subLTSlemma)
+            have c6:"LTS_is_reachable  ({(Concat q (Star r), va, Concat q' (Star r)) |q va q'. (q, va, q') \<in> fst (trans2LTS r v)} \<union> fst (trans2LTS r v))
+                    ((insert (Star r, Concat r (Star r)) (insert (Concat \<epsilon> (Star r), Star r) {(Concat q (Star r), Concat q' (Star r)) |q q'. (q, q') \<in> snd (trans2LTS r v)})))
                     (Concat r (Star r)) x (Concat \<epsilon> (Star r))"
-              using c5 by (metis (no_types, lifting) Pair_inject Un_absorb Un_insert_right prod.collapse subLTSlemma)
+              using c5 by (metis (no_types, lifting) Un_insert_right subLTSlemma sup_idem) 
             have c7:"LTS_is_reachable
-                    ({(Concat q (Star r), va, Concat q' (Star r)) |q va q'. (q, va, q') \<in> fst (trans2LTS r v)},
-                    insert (Star r, \<epsilon>) (insert (Star r, Concat r (Star r)) (insert (Concat \<epsilon> (Star r), Star r) {(Concat q (Star r), Concat q' (Star r)) |q q'. (q, q') \<in> snd (trans2LTS r v)})))
+                    ({(Concat q (Star r), va, Concat q' (Star r)) |q va q'. (q, va, q') \<in> fst (trans2LTS r v)})
+                    (insert (Star r, \<epsilon>) (insert (Star r, Concat r (Star r)) (insert (Concat \<epsilon> (Star r), Star r) {(Concat q (Star r), Concat q' (Star r)) |q q'. (q, q') \<in> snd (trans2LTS r v)})))
                     (Concat r (Star r)) x (Concat \<epsilon> (Star r))"
-              by (metis (no_types, lifting) Un_insert_right c2 fst_conv snd_conv subLTSlemma sup.idem)
+              by (metis (no_types, lifting) Un_absorb Un_insert_right c2 subLTSlemma)
             have c8:"LTS_is_reachable
-                    ({(Concat q (Star r), va, Concat q' (Star r)) |q va q'. (q, va, q') \<in> fst (trans2LTS r v)},
-                    insert (Star r, \<epsilon>) (insert (Star r, Concat r (Star r)) (insert (Concat \<epsilon> (Star r), Star r) {(Concat q (Star r), Concat q' (Star r)) |q q'. (q, q') \<in> snd (trans2LTS r v)})))
+                    ({(Concat q (Star r), va, Concat q' (Star r)) |q va q'. (q, va, q') \<in> fst (trans2LTS r v)})
+                    (insert (Star r, \<epsilon>) (insert (Star r, Concat r (Star r)) (insert (Concat \<epsilon> (Star r), Star r) {(Concat q (Star r), Concat q' (Star r)) |q q'. (q, q') \<in> snd (trans2LTS r v)})))
                     (Star r) x (Concat \<epsilon> (Star r))"
               using c1 c7 by (smt (z3) LTS_Step1 insertI1 insert_commute snd_conv)
             have c9:"LTS_is_reachable
-                    ({(Concat q (Star r), va, Concat q' (Star r)) |q va q'. (q, va, q') \<in> fst (trans2LTS r v)},
-                    insert (Star r, \<epsilon>) (insert (Star r, Concat r (Star r)) (insert (Concat \<epsilon> (Star r), Star r) {(Concat q (Star r), Concat q' (Star r)) |q q'. (q, q') \<in> snd (trans2LTS r v)})))
+                    ({(Concat q (Star r), va, Concat q' (Star r)) |q va q'. (q, va, q') \<in> fst (trans2LTS r v)})
+                    (insert (Star r, \<epsilon>) (insert (Star r, Concat r (Star r)) (insert (Concat \<epsilon> (Star r), Star r) {(Concat q (Star r), Concat q' (Star r)) |q q'. (q, q') \<in> snd (trans2LTS r v)})))
                     (Concat \<epsilon> (Star r)) [] (Star r)"
-              by (metis (no_types, lifting) LTS_Empty LTS_Step1 insertCI snd_conv)
+              by (smt (verit, best) LTS_Empty LTS_Step1 insertI1 insert_commute)
             have c10:"LTS_is_reachable
-                    ({(Concat q (Star r), va, Concat q' (Star r)) |q va q'. (q, va, q') \<in> fst (trans2LTS r v)},
-                    insert (Star r, \<epsilon>) (insert (Star r, Concat r (Star r)) (insert (Concat \<epsilon> (Star r), Star r) {(Concat q (Star r), Concat q' (Star r)) |q q'. (q, q') \<in> snd (trans2LTS r v)})))
+                    ({(Concat q (Star r), va, Concat q' (Star r)) |q va q'. (q, va, q') \<in> fst (trans2LTS r v)})
+                    (insert (Star r, \<epsilon>) (insert (Star r, Concat r (Star r)) (insert (Concat \<epsilon> (Star r), Star r) {(Concat q (Star r), Concat q' (Star r)) |q q'. (q, q') \<in> snd (trans2LTS r v)})))
                     (Star r) x (Star r)"
               using c8 c9 joinLTSlemma by fastforce              
             thus ?thesis using a3 c10 joinLTSlemma 
@@ -555,7 +501,15 @@ next
         qed
       qed
     qed
-    subgoal for x sorry
+    subgoal for x 
+    proof -
+      assume a1:"sem_reg r v = {w. LTS_is_reachable (fst (trans2LTS r v)) (snd (trans2LTS r v)) r w \<epsilon>}"
+      assume a2:"LTS_is_reachable {(Concat q (Star r), va, Concat q' (Star r)) |q va q'. (q, va, q') \<in> fst (trans2LTS r v)}
+                 (insert (Star r, \<epsilon>) (insert (Star r, Concat r (Star r)) (insert (Concat \<epsilon> (Star r), Star r) {(Concat q (Star r), Concat q' (Star r)) |q q'. (q, q') \<in> snd (trans2LTS r v)})))
+                 (Star r) x \<epsilon>"
+      show "x \<in> star {w. LTS_is_reachable (fst (trans2LTS r v)) (snd (trans2LTS r v)) r w \<epsilon>}"
+        sorry
+    qed
     done
 next
   case (Ques r)
@@ -564,28 +518,28 @@ next
     apply auto 
     subgoal 
     proof -
-      assume "sem_reg r v = {w. LTS_is_reachable (trans2LTS r v) r w \<epsilon>}"
-      show "LTS_is_reachable (fst (trans2LTS r v), insert (Ques r, \<epsilon>) (insert (Ques r, r) (snd (trans2LTS r v)))) (Ques r) [] \<epsilon>"
-        by (metis LTS_Empty LTS_Step1 insertI1 snd_conv)
+      assume "sem_reg r v = {w. LTS_is_reachable (fst (trans2LTS r v)) (snd (trans2LTS r v)) r w \<epsilon>}"
+      show "LTS_is_reachable (fst (trans2LTS r v)) (insert (Ques r, \<epsilon>) (insert (Ques r, r) (snd (trans2LTS r v)))) (Ques r) [] \<epsilon>"
+        by (metis LTS_Empty LTS_Step1 insertI1)
     qed
     subgoal for x
     proof -
-      assume a1:"sem_reg r v = {w. LTS_is_reachable (trans2LTS r v) r w \<epsilon>}"
-      assume a2:"LTS_is_reachable (trans2LTS r v) r x \<epsilon>"
-      show "LTS_is_reachable (fst (trans2LTS r v), insert (Ques r, \<epsilon>) (insert (Ques r, r) (snd (trans2LTS r v)))) (Ques r) x \<epsilon>"
+      assume a1:"sem_reg r v = {w. LTS_is_reachable (fst (trans2LTS r v)) (snd (trans2LTS r v)) r w \<epsilon>}"
+      assume a2:"LTS_is_reachable (fst (trans2LTS r v)) (snd (trans2LTS r v)) r x \<epsilon>"
+      show "LTS_is_reachable (fst (trans2LTS r v)) (insert (Ques r, \<epsilon>) (insert (Ques r, r) (snd (trans2LTS r v)))) (Ques r) x \<epsilon>"
       proof -
-        from a2 have c1:"LTS_is_reachable (fst (trans2LTS r v), insert (Ques r, \<epsilon>) (insert (Ques r, r) (snd (trans2LTS r v)))) r x \<epsilon>"
+        from a2 have c1:"LTS_is_reachable (fst (trans2LTS r v)) (insert (Ques r, \<epsilon>) (insert (Ques r, r) (snd (trans2LTS r v)))) r x \<epsilon>"
           apply(induction rule:LTS_is_reachable.induct)
           subgoal 
             by auto
-          subgoal for q lts l q'
+          subgoal for q q'' \<Delta>' \<Delta> l q'
             apply auto
             by (smt (verit, best) LTS_Step1 Un_insert_right subLTSlemma sup_idem)
-          subgoal for a q lts w q'
+          subgoal for a q \<Delta> \<Delta>' w q'
             apply auto
             by (metis Un_insert_right boolean_algebra_cancel.sup0 subLTSlemma)
           done
-        have "LTS_is_reachable (fst (trans2LTS r v), insert (Ques r, \<epsilon>) (insert (Ques r, r) (snd (trans2LTS r v)))) (Ques r) x \<epsilon>"
+        have "LTS_is_reachable (fst (trans2LTS r v)) (insert (Ques r, \<epsilon>) (insert (Ques r, r) (snd (trans2LTS r v)))) (Ques r) x \<epsilon>"
           using c1
           by (smt (verit, best) LTS_Step1 insertI1 insert_commute snd_conv)
         thus ?thesis by auto
@@ -593,18 +547,39 @@ next
     qed
     subgoal for x
     proof -
-      assume a1:"sem_reg r v = {w. LTS_is_reachable (trans2LTS r v) r w ε}"
-      assume a2:"LTS_is_reachable (fst (trans2LTS r v), insert (Ques r, ε) (insert (Ques r, r) (snd (trans2LTS r v)))) (Ques r) x ε"
+      assume a1:"sem_reg r v = {w. LTS_is_reachable (fst (trans2LTS r v)) (snd (trans2LTS r v)) r w \<epsilon>}"
+      assume a2:"LTS_is_reachable (fst (trans2LTS r v)) (insert (Ques r, \<epsilon>) (insert (Ques r, r) (snd (trans2LTS r v)))) (Ques r) x \<epsilon>"
       assume a3:"x \<noteq> []" 
-      from a1 a2 a3 show "LTS_is_reachable (trans2LTS r v) r x ε"
+      from a1 a2 a3 show "LTS_is_reachable (fst (trans2LTS r v)) (snd (trans2LTS r v)) r x \<epsilon>"
       proof(induction x)
         case Nil
           then show ?case apply auto done
         next
           case (Cons a x)
-          then show ?case apply simp 
-          
+          then show ?case 
+            apply simp 
+          proof - 
+            assume a4:"LTS_is_reachable (fst (trans2LTS r v)) (insert (Ques r, \<epsilon>) (insert (Ques r, r) (snd (trans2LTS r v)))) (Ques r) (a # x) \<epsilon>" 
+            have c1:"LTS_is_reachable (fst (trans2LTS r v)) (snd (trans2LTS r v)) \<epsilon> x \<epsilon> \<Longrightarrow> x=[]" apply (rule LTS_is_reachable.cases) apply auto 
+              subgoal for q'' proof -
+                assume a1:"(\<epsilon>, q'') \<in> snd (trans2LTS r v)"
+                assume a2:"\<epsilon> \<noteq> q''"
+                from a1 have c1:"q'' = \<epsilon>" by auto
+                from a2 c1 have "False" by auto then show ?thesis by auto
+              qed
+              subgoal for a w q'' \<sigma> proof -
+                assume a1:"(\<epsilon>, \<sigma>, q'') \<in> fst (trans2LTS r v)" 
+                then show "False" by (induct r) auto
+              qed
+              done
+            from c1 have "LTS_is_reachable (fst (trans2LTS r v)) ({(Ques r, \<epsilon>)} \<union> (snd (trans2LTS r v))) (Ques r) x \<epsilon> \<Longrightarrow> x = []"
+              apply auto
+              apply (rule LTS_is_reachable.cases)
+              apply simp
+              subgoal for \<Delta> \<Delta>' q by auto
+              subgoal for q q'' \<Delta>' \<Delta> l q' 
           qed
       qed
+      done
   qed
 end
